



Figure 5.3 Various methods of numerical integration.

These three integration rules are based on approximating the target function (integrand) to the zeroth-, first- and second-degree polynomial, respectively. Since the first two integrations are obvious, we are going to derive just Simpson's rule (5.5.4). For simplicity, we shift the graph of $f(x)$ by $-x_k$ along the x axis, or, equivalently, make the variable substitution $t = x - x_k$ so that the abscissas of the three points on the curve of $f(x)$ change from $x = \{x_k - h, x_k, x_k + h\}$ to $t = \{-h, 0, +h\}$. Then, in order to find the coefficients of the second-degree polynomial

$$p_2(t) = c_1 t^2 + c_2 t + c_3 \quad (5.5.5)$$

matching the points $(-h, f_{k-1})$, $(0, f_k)$, $(+h, f_{k+1})$, we should solve the following set of equations:

$$\begin{aligned} p_2(-h) &= c_1(-h)^2 + c_2(-h) + c_3 = f_{k-1} \\ p_2(0) &= c_1 0^2 + c_2 0 + c_3 = f_k \\ p_2(+h) &= c_1(+h)^2 + c_2(+h) + c_3 = f_{k+1} \end{aligned}$$

to determine the coefficients c_1 , c_2 , and c_3 as

$$\begin{aligned} c_3 &= f_k, & c_2 &= \frac{f_{k+1} - f_{k-1}}{2h}, & c_1 &= \frac{1}{h^2} \left(\frac{f_{k+1} + f_{k-1}}{2} - f_k \right) \end{aligned}$$

Integrating the second-degree polynomial (5.5.5) with these coefficients from $t = -h$ to $t = h$ yields

$$\begin{aligned} \int_{-h}^h p_2(t) dt &= \frac{1}{3} c_1 t^3 + \frac{1}{2} c_2 t^2 + c_3 t \Big|_{-h}^h = \frac{2}{3} c_1 h^3 + 2c_3 h \\ &= \frac{2h}{3} \left(\frac{f_{k+1} + f_{k-1}}{2} - f_k + 3f_k \right) = \frac{h}{3} (f_{k-1} + 4f_k + f_{k+1}) \end{aligned}$$

This is the Simpson integration formula (5.5.4).

Now, as a preliminary work toward diagnosing the errors of the above integration formulas, we take the Taylor series expansion of the integral function

$$g(x) = \int_{x_k}^x f(t) dt \quad \text{with } g'(x) = f(x), \quad g^{(2)}(x) = f'(x), \quad g^{(3)}(x) = f^{(2)}(x) \quad (5.5.6)$$

about the lower bound x_k of the integration interval to write

$$g(x) = g(x_k) + g'(x_k)(x - x_k) + \frac{1}{2} g^{(2)}(x_k)(x - x_k)^2 + \frac{1}{3!} g^{(3)}(x_k)(x - x_k)^3 + \dots$$

Substituting Eq. (5.5.6) together with $x = x_{k+1}$ and $x_{k+1} - x_k = h$ into this yields

$$\int_{x_k}^{x_{k+1}} f(x) dx = 0 + hf(x_k) + \frac{h^2}{2} f'(x_k) + \frac{h^3}{3!} f^{(2)}(x_k) + \frac{h^4}{4!} f^{(3)}(x_k) + \frac{h^5}{5!} f^{(4)}(x_k) + \dots \quad (5.5.7)$$

First, for the error analysis of the midpoint rule, we substitute x_{k-1} and $-h = x_{k-1} - x_k$ in place of x_{k+1} and h in this equation to write

$$\int_{x_k}^{x_{k-1}} f(x) dx = 0 - hf(x_k) + \frac{h^2}{2} f'(x_k) - \frac{h^3}{3!} f^{(2)}(x_k) + \frac{h^4}{4!} f^{(3)}(x_k) - \frac{h^5}{5!} f^{(4)}(x_k) + \dots$$

and subtract this equation from Eq. (5.5.7) to write

$$\begin{aligned} \int_{x_k}^{x_{k+1}} f(x) dx - \int_{x_k}^{x_{k-1}} f(x) dx &= \int_{x_k}^{x_{k+1}} f(x) dx + \int_{x_{k-1}}^{x_k} f(x) dx \\ &= \int_{x_{k-1}}^{x_{k+1}} f(x) dx = 2hf(x_k) + \frac{2h^3}{3!} f^{(2)}(x_k) + \frac{2h^5}{5!} f^{(4)}(x_k) + \dots \quad (5.5.8) \end{aligned}$$

Substituting x_k and $x_{mk} = (x_k + x_{k+1})/2$ in place of x_{k-1} and x_k in this equation and noting that $x_{k+1} - x_{mk} = x_{mk} - x_k = h/2$, we obtain

$$\begin{aligned} \int_{x_k}^{x_{k+1}} f(x) dx &= hf(x_{mk}) + \frac{h^3}{3 \times 2^3} f^{(2)}(x_{mk}) \\ &\quad + \frac{h^5}{5 \times 4 \times 3 \times 2^5} f^{(4)}(x_{mk}) + \dots \end{aligned}$$

$$\int_{x_k}^{x_{k+1}} f(x) dx - hf(x_{mk}) = \frac{h^3}{24} f^{(2)}(x_{mk}) + \frac{h^5}{1920} f^{(4)}(x_{mk}) + \dots = O(h^3) \quad (5.5.9)$$